

DSA 8505: Bayesian Statistics

Marking Scheme

Master of Science in Data Science & Analytics

14th Feb 2025

1. Bayesian Credible Interval

Step 1: Understanding the Posterior Distribution

We are given that the posterior distribution of θ is:

$$\theta|x \sim \mathcal{N}(\mu, \sigma^2).$$

This means that θ follows a normal distribution with:

- **Mean:** μ (posterior mean),
- **Variance:** σ^2 (posterior variance),
- **Standard deviation:** σ (posterior standard deviation).

Step 2: Definition of Equal-Tailed Credible Interval

The **90% equal-tailed credible interval** for θ is determined by finding values θ_L and θ_U such that:

$$P(\theta_L \leq \theta \leq \theta_U | x) = 0.90.$$

Since the normal distribution is symmetric, the **equal-tailed** interval ensures that 5% of the probability mass is in each tail:

$$P(\theta \leq \theta_L | x) = 0.05, \quad P(\theta \geq \theta_U | x) = 0.05.$$

This means we need to find the **5th percentile** and **95th percentile** of the normal posterior distribution.

Step 3: Computing the Credible Interval

For a **standard normal distribution** $Z \sim \mathcal{N}(0, 1)$, the **critical values** for a **90% interval** are:

$$z_{\alpha/2} = z_{0.05} \approx -1.645, \quad z_{1-\alpha/2} = z_{0.95} \approx 1.645.$$

Since θ follows $\mathcal{N}(\mu, \sigma^2)$, we apply the transformation:

$$\theta_L = \mu + z_{0.05} \cdot \sigma = \mu - 1.645\sigma.$$

$$\theta_U = \mu + z_{0.95} \cdot \sigma = \mu + 1.645\sigma.$$

Thus, the **90% credible interval** for θ is:

$$(\mu - 1.645\sigma, \mu + 1.645\sigma).$$

Final Answer

$$\theta \in (\mu - 1.645\sigma, \mu + 1.645\sigma).$$

2. Bayesian Updating with Beta Prior

Step 1: Identify the Prior Distribution

The prior distribution for θ is given as:

$$\theta \sim \text{Beta}(\alpha, \beta) = \text{Beta}(3, 3).$$

This means the prior probability density function (PDF) is:

$$p(\theta) \propto \theta^{\alpha-1} (1-\theta)^{\beta-1}, \quad 0 \leq \theta \leq 1.$$

Step 2: Identify the Likelihood Function

Since the outcome of each die roll is independent and follows a **Bernoulli distribution** (success: rolling a six), the likelihood function for observing **6 sixes in 15 rolls** follows a **Binomial distribution**:

$$p(x|\theta) = \binom{n}{x} \theta^x (1-\theta)^{n-x}.$$

Substituting $x = 6$ and $n = 15$:

$$p(6|\theta) \propto \theta^6 (1-\theta)^9.$$

Step 3: Compute the Posterior Distribution

Using Bayes' theorem:

$$p(\theta|x) \propto p(\theta) \cdot p(x|\theta).$$

Substituting the **prior** and **likelihood**:

$$p(\theta|x) \propto \theta^{(3-1)} (1-\theta)^{(3-1)} \cdot \theta^6 (1-\theta)^9.$$

$$p(\theta|x) \propto \theta^{2-1} (1-\theta)^{2-1} \cdot \theta^6 \cdot (1-\theta)^{9-6}$$

$$p(\theta|x) \propto \theta^{(3+6-1)}(1-\theta)^{(3+9-1)}$$

$$p(\theta|x) \propto \theta^8(1-\theta)^{11} \quad \checkmark$$

$$p(\theta|x) \propto \theta^{\alpha-1}(1-\theta)^{\beta-1}$$

$$\alpha-1=8 \quad \alpha=9 \quad \beta-1=11 \quad \beta=12$$

$$\dots \pi(\theta|x) \sim B(9,12)$$

Comparing with the **Beta distribution form**:

$$\text{Beta}(\alpha', \beta') \propto \theta^{\alpha'-1}(1-\theta)^{\beta'-1}.$$

We identify that:

$$\alpha' = 3 + 6 = 9, \quad \beta' = 3 + 9 = 12.$$

Final Answer: Posterior Distribution

$$\theta|x \sim \text{Beta}(9, 12).$$

This is the **updated belief** about θ after observing the data.

3. Bayes Estimators

Given:

$$\pi(\theta|x) \sim N(10, 16).$$

$$E(\theta|x) = \mu = 10$$

- (a) **Bayes estimator under squared error loss** [1 mark] The Bayes estimator under squared error loss is the posterior mean:

$$\hat{\theta}_{\text{Bayes}} = E[\theta|x] = 10.$$

- (b) **Bayes estimator under absolute error loss** [1 mark] The Bayes estimator under absolute error loss is the posterior median:

$$\hat{\theta}_{\text{Bayes}} = \text{Median}(\theta|x) = 10.$$

Since the normal distribution is symmetric, the mean and median are the same.

4. MAP Estimation vs. Bayes Estimator

- (a) **Difference between MAP and Bayes estimator** - The MAP estimate is the mode (most probable value), which is $\theta = 6$. - The Bayes estimator under squared error loss is the posterior mean, which may be different from the mode.
- (b) **Choosing estimate under squared error loss** - Since squared error loss minimizes expected error, we choose the posterior mean $\hat{\theta} = 4.5$.

5. Bayesian Estimation with Normal Prior and Likelihood

- (a) **Derivation of posterior distribution**

We are given:

- Prior:**

$$\theta \sim N(\mu_0, \sigma_0^2) \quad \checkmark$$

- Likelihood:**

$$x|\theta \sim N(\mu, \sigma^2) \quad \checkmark$$

\cdot posterior $\theta|x$?? $\pi(\theta|x) \propto p(\theta) \pi(x|\theta)$

Step 1: Compute the Posterior using Bayes' Theorem

By Bayes' theorem, the posterior distribution is proportional to the product of the prior and the likelihood:

$$\pi(\theta|x) \propto p(x|\theta)\pi(\theta).$$

Expanding each term:

- **Prior distribution:**

$$\pi(\theta) = \frac{1}{\sqrt{2\pi\sigma_0^2}} \exp\left(-\frac{(\theta - \mu_0)^2}{2\sigma_0^2}\right).$$

- **Likelihood function:**

$$p(x|\theta) = \frac{1}{\sqrt{2\pi\sigma^2}} \exp\left(-\frac{(x - \theta)^2}{2\sigma^2}\right).$$

Taking the product:

$$\pi(\theta|x) \propto \exp\left(-\frac{(\theta - \mu_0)^2}{2\sigma_0^2} - \frac{(x - \theta)^2}{2\sigma^2}\right).$$

$$\pi(\theta) \propto \exp\left[-\frac{1}{2} \frac{(\theta - \mu_0)^2}{\sigma_0^2}\right]$$

$$p(x|\theta) \propto \exp\left[-\frac{1}{2} \frac{(x - \theta)^2}{\sigma^2}\right]$$

$$\pi(\theta|x) \propto \pi(\theta) \cdot p(x|\theta)$$

$$e^a e^b = e^{a+b}$$

Step 2: Completing the Square

Expanding the exponents:

$$-\frac{(\theta - \mu_0)^2}{2\sigma_0^2} - \frac{(x - \theta)^2}{2\sigma^2}.$$

Rewriting each quadratic term:

$$-\frac{\theta^2 - 2\mu_0\theta + \mu_0^2}{2\sigma_0^2} - \frac{x^2 - 2x\theta + \theta^2}{2\sigma^2}.$$

Rearranging:

$$-\frac{\theta^2}{2\sigma_0^2} + \frac{\mu_0\theta}{\sigma_0^2} - \frac{\mu_0^2}{2\sigma_0^2} - \frac{x^2}{2\sigma^2} + \frac{x\theta}{\sigma^2} - \frac{\theta^2}{2\sigma^2}.$$

Factor out θ^2 :

$$-\theta^2 \left(\frac{1}{2\sigma_0^2} + \frac{1}{2\sigma^2} \right) + \theta \left(\frac{\mu_0}{\sigma_0^2} + \frac{x}{\sigma^2} \right) + (\text{constant terms}).$$

Since this is the exponent of a normal distribution, the posterior mean and variance are:

Step 3: Compute Posterior Mean and Variance

- ****Posterior Variance**:**

$$\sigma_{\text{post}}^2 = \frac{1}{\frac{1}{\sigma_0^2} + \frac{1}{\sigma^2}}$$

- ****Posterior Mean**:**

$$\mu_{\text{post}} = \sigma_{\text{post}}^2 \left(\frac{\mu_0}{\sigma_0^2} + \frac{x}{\sigma^2} \right).$$

Substituting σ_{post}^2 :

$$\mu_{\text{post}} = \frac{\frac{\mu_0}{\sigma_0^2} + \frac{x}{\sigma^2}}{\frac{1}{\sigma_0^2} + \frac{1}{\sigma^2}}.$$

$$ax^2 + bx + \frac{b^2}{4a}$$

$$ax^2 + bx + \frac{b^2}{4a}$$

$$-\frac{1}{2} \left[\frac{(x - \mu_{\text{post}})^2}{\sigma_{\text{post}}^2} \right]$$

$$\sigma_{\text{post}}^2 = \frac{1}{\frac{1}{\sigma_0^2} + \frac{1}{\sigma^2}}$$

$$\pi(\theta|x) \sim \mathcal{N}(\mu_{\text{post}}, \sigma_{\text{post}}^2)$$

Therefore, the posterior distribution is:

$$\theta|x \sim N\left(\frac{\frac{\mu_0}{\sigma_0^2} + \frac{x}{\sigma^2}}{\frac{1}{\sigma_0^2} + \frac{1}{\sigma^2}}, \frac{1}{\frac{1}{\sigma_0^2} + \frac{1}{\sigma^2}}\right).$$

- (b) **Posterior mean minimizes squared error loss** We want to show that the **posterior mean** is the Bayesian estimator under **squared error loss**. That is, given the loss function:

$$L(\theta, \hat{\theta}) = (\theta - \hat{\theta})^2,$$

we aim to minimize the expected posterior loss.

$$R(\hat{\theta}) = E_{\pi}[(\theta - \hat{\theta})^2|x]$$

Step 1: Expected Posterior Loss Function

The expected squared error loss is:

$$R(\hat{\theta}) = E_{\pi}[(\theta - \hat{\theta})^2|x].$$

Expanding the expectation:

$$R(\hat{\theta}) = \int_{-\infty}^{\infty} (\theta - \hat{\theta})^2 \pi(\theta|x) d\theta.$$

Step 2: Expanding the Integral

Expanding the squared term:

$$(\theta - \hat{\theta})^2 = (\theta - E[\theta|x] + E[\theta|x] - \hat{\theta})^2.$$

Expanding further:

$$E_{\pi}[(\theta - \hat{\theta})^2] = E_{\pi}[(\theta - E[\theta|x])^2] + 2E_{\pi}[(\theta - E[\theta|x])(E[\theta|x] - \hat{\theta})] + E_{\pi}[(E[\theta|x] - \hat{\theta})^2].$$

Step 3: Taking Expectation

Taking expectation on both sides:

$$E_{\pi}[(\theta - \hat{\theta})^2|x] = E_{\pi}[(\theta - E[\theta|x])^2|x] + 2E_{\pi}[(\theta - E[\theta|x])(E[\theta|x] - \hat{\theta})|x] + (E[\theta|x] - \hat{\theta})^2.$$

The second term is zero because:

$$E_{\pi}[(\theta - E[\theta|x]) = 0.$$

This simplifies to:

$$E_{\pi}[(\theta - \hat{\theta})^2|x] = E_{\pi}[(\theta - E[\theta|x])^2|x] + (E[\theta|x] - \hat{\theta})^2.$$

$$X = \{0, 5, 10\}$$

$$E(X) = \text{mean} = 5$$

$$E(\theta|x) - \hat{\theta} = 0 \Rightarrow \hat{\theta} = E(\theta|x)$$

$$E_{\pi}((\theta - \hat{\theta})|x) = 0 \quad \therefore E(\theta|x) - \hat{\theta} = 0 \\ \hat{\theta} = E(\theta|x) \#$$

Step 4: Minimizing the Risk Function

Since the first term is independent of $\hat{\theta}$, the only term affecting the choice of $\hat{\theta}$ is $(E[\theta|x] - \hat{\theta})^2$, which is minimized when:

$$\hat{\theta} = E[\theta|x].$$

Thus, the posterior mean:

$$\hat{\theta}_{\text{Bayes}} = E[\theta|x]$$

minimizes the expected squared error loss.

Since the squared error loss function penalizes deviations quadratically, the **optimal estimator is the posterior mean**. Hence, the **Bayesian estimator under squared error loss is the posterior mean**.

$$\hat{\theta}_{\text{Bayes}} = E[\theta|x].$$

(c) **Compute Bayesian estimator** Given:

$$\theta \sim N(6, 2), \quad x|\theta \sim N(12, 3),$$

we compute the posterior mean:

$$\mu_{\text{post}} = \frac{\frac{6}{2} + \frac{12}{3}}{\frac{1}{2} + \frac{1}{3}}.$$

Computing step by step:

$$\frac{6}{2} = 3, \quad \frac{12}{3} = 4, \quad \frac{1}{2} = 0.5, \quad \frac{1}{3} = 0.3333.$$

$$\mu_{\text{post}} = \frac{3 + 4}{0.5 + 0.3333} = \frac{7}{0.8333} = 8.4.$$

$$\theta|x \sim N(\mu_{\text{post}}, \sigma_{\text{post}}^2)$$